hax-lib/proof-libs/lean/Hax/core_models/epilogue/num.lean
@@ -10,20 +10,20 @@ def rotate_left (x : u32) (n : u32) : RustM u32 :=
   pure (UInt32.ofBitVec (BitVec.rotateLeft x.toBitVec n.toNat))
 
 @[spec]
-def from_le_bytes (x : Vector u8 4) : RustM u32 :=
-  pure (x[0].toUInt32
-  + (x[1].toUInt32 <<< 8)
-  + (x[2].toUInt32 <<< 16)
-  + (x[3].toUInt32 <<< 24))
+def from_le_bytes (x : RustArray u8 4) : RustM u32 :=
+  pure (x.toVec[0].toUInt32
+  + (x.toVec[1].toUInt32 <<< 8)
+  + (x.toVec[2].toUInt32 <<< 16)
+  + (x.toVec[3].toUInt32 <<< 24))
 
 @[spec]
-def to_le_bytes (x : u32) : RustM (Vector u8 4) :=
-  pure #v[
+def to_le_bytes (x : u32) : RustM (RustArray u8 4) :=
+  pure (.ofVec #v[
     (x % 256).toUInt8,
     (x >>> 8 % 256).toUInt8,
     (x >>> 16 % 256).toUInt8,
     (x >>> 24 % 256).toUInt8,
-  ]
+  ])
 
 end core_models.num.Impl_8
 
